PREFIX demo: <http://prez.demo/>
PREFIX skos: <http://www.w3.org/2004/02/skos/core#>

demo:fuseki
    a skos:Concept ;
    skos:inScheme demo:cs ;
    skos:prefLabel "Fuseki" ;
	skos:definition "Apache Jena Fuseki is a SPARQL server. It can run as a standalone server, or embedded in an application."
.

demo:prez
    a skos:Concept ;
    skos:inScheme demo:cs ;
    skos:prefLabel "Prez" ;
	skos:definition "Prez is an open source web application API that delivers 'profiles of Knowledge Graph data'."
.

demo:prez-ui
    a skos:Concept ;
    skos:inScheme demo:cs ;
    skos:prefLabel "Prez UI" ;
	skos:definition "Prez UI is the front end of Prez - a linked data API - and is a suite of packages to interact with and render RDF in JavaScript."
.

demo:cs
    a skos:ConceptScheme ;
    skos:hasTopConcept
        demo:fuseki ,
        demo:prez ,
        demo:prez-ui ;
    skos:prefLabel "Demo Concept Scheme" ;
.
